mrdts-new/Observed-remove_set_eff/App_new.fst
@@ -8,13 +8,19 @@ module S' = Set_extended
 
 let cf = (int * bool)
 
+// concrete state of ew flag
+type concrete_st_e = M.t nat cf // (replica_id, ctr, flag) //replica ids are unique
+
 // the concrete state type
-type concrete_st = M.t nat (M.t nat cf) // element ->
+type concrete_st = M.t nat concrete_st_e // element ->
                                        //    replica ID -> 
                                        //       (ctr, flag) //elements & replica ids are unique
 
+// init state of ew flag
+let init_st_e : concrete_st_e = M.const (0, false)
+
 // init state
-let init_st : concrete_st = M.const (M.const (0, false))
+let init_st : concrete_st = M.const init_st_e
 
 let sel_e (s:concrete_st) e = if M.contains s e then M.sel s e else (M.const (0, false))
 
@@ -23,11 +29,14 @@ let sel_id (s:M.t nat cf) id = if M.contains s id then M.sel s id else (0, false
 let ele_id (s:concrete_st) (e id:nat) =
   M.contains s e /\ M.contains (sel_e s e) id
 
+// equivalence relation of ew flag
+let eq_e (a b:concrete_st_e) =
+  (forall id. (M.contains a id = M.contains b id) /\ (sel_id a id == sel_id b id))
+
 // equivalence between 2 concrete states
 let eq (a b:concrete_st) =
   (forall e. M.contains a e = M.contains b e) /\
-  (forall e. M.contains a e ==> (forall id. M.contains (sel_e a e) id = M.contains (sel_e b e) id /\ 
-                                  sel_id (sel_e a e) id == sel_id (sel_e b e) id))
+  (forall e. M.contains a e ==> eq_e (sel_e a e) (sel_e b e))
 
 let symmetric (a b:concrete_st) 
   : Lemma (requires eq a b)
@@ -46,17 +55,6 @@ type app_op_t:eqtype =
   |Add : nat -> app_op_t
   |Rem : nat -> app_op_t
 
-type op_t = pos (*timestamp*) & (nat (*replica ID*) & app_op_t)
-
-//let distinct_ops (op1 op2:op_t) = fst op1 =!= fst op2
-
-let get_rid (_,(rid,_)) = rid
-
-type rc_res =
-  |Fst_then_snd //o1 -> o2
-  |Snd_then_fst //o2 -> o1
-  |Either
-
 let get_ele (o:op_t) : nat =
   match snd (snd o) with
   |Add e -> e
@@ -68,9 +66,6 @@ let do (s:concrete_st) (o:op_t) : concrete_st =
   |(_, (rid, Add e)) -> M.upd s e (M.upd (sel_e s e) rid (fst (sel_id (sel_e s e) rid) + 1, true))
   |(_, (rid, Rem e)) -> M.iter_upd (fun k v -> if k = e then ((M.map_val (fun (c,f) -> (c, false))) v) else v) s
 
-let commutes_with (o1 o2:op_t) =
-  forall s. eq (do (do s o1) o2) (do (do s o2) o1)
-  
 //conflict resolution
 let rc (o1:op_t) (o2:op_t(*{distinct_ops o1 o2}*)) =
   match snd (snd o1), snd (snd o2) with
@@ -124,135 +119,145 @@ let cond_comm (o1:op_t) (o2:op_t{~ (Either? (rc o1 o2))}) (o3:op_t) =
   if Rem? (snd (snd o3)) && get_ele o1 = get_ele o3 then true else false
 
 #push-options "--z3rlimit 100 --max_ifuel 3 --split_queries on_failure"
-//#push-options "--z3rlimit 50 --max_ifuel 3"
+let cond_comm_base (s:concrete_st) (o1 o2 o3:op_t)
+  : Lemma (requires distinct_ops o1 o2 /\ ~ (Either? (rc o1 o2)) /\ cond_comm o1 o2 o3)
+          (ensures eq (do (do (do s o1) o2) o3) (do (do (do s o2) o1) o3)) = ()
 
-// let cond_comm_base (s:concrete_st) (o1 o2 o3:op_t)
-//   : Lemma (requires distinct_ops o1 o2 /\ ~ (Either? (rc o1 o2)) /\ cond_comm o1 o2 o3)
-//           (ensures eq (do (do (do s o1) o2) o3) (do (do (do s o2) o1) o3)) = ()
-
-// let cond_comm_ind (s:concrete_st) (o1 o2 o3 o:op_t) (l:log)
-//   : Lemma (requires distinct_ops o1 o2 /\ ~ (Either? (rc o1 o2)) /\ cond_comm o1 o2 o3 /\
-//                     eq (do (apply_log (do (do s o1) o2) l) o3) (do (apply_log (do (do s o2) o1) l) o3))
-//           (ensures eq (do (do (apply_log (do (do s o1) o2) l) o) o3) (do (do (apply_log (do (do s o2) o1) l) o) o3)) = ()
+let cond_comm_ind (s:concrete_st) (o1 o2 o3 o:op_t) (l:log)
+  : Lemma (requires distinct_ops o1 o2 /\ ~ (Either? (rc o1 o2)) /\ cond_comm o1 o2 o3 /\
+                    eq (do (apply_log (do (do s o1) o2) l) o3) (do (apply_log (do (do s o2) o1) l) o3))
+          (ensures eq (do (do (apply_log (do (do s o1) o2) l) o) o3) (do (do (apply_log (do (do s o2) o1) l) o) o3)) = ()
           
 /////////////////////////////////////////////////////////////////////////////
 
 // Merge commutativity
- let merge_comm (l a b:concrete_st)
+let merge_comm (l a b:concrete_st)
    : Lemma (ensures (eq (merge l a b) (merge l b a))) = ()
 
 // Merge idempotence
- let merge_idem (s:concrete_st)
+let merge_idem (s:concrete_st)
    : Lemma (ensures eq (merge s s s) s) = ()
 
 (*Two OP RC*)
 //////////////// 
-let rc_ind_right (l a b:concrete_st) (o1 o2' o2:op_t)
+let rc_ind_right' (l a b:concrete_st) (o1 o2' o2:op_t)
    : Lemma (requires Fst_then_snd? (rc o1 o2) /\
-                     eq (merge l (do a o1) (do b o2)) (do (merge l (do a o1) b) o2))
+                     eq (merge l (do a o1) (do b o2)) (do (merge l (do a o1) b) o2) /\
+                     (forall e. eq_e (sel_e (merge l (do a o1) (do (do b o2') o2)) e) (sel_e (do (merge l (do a o1) (do b o2')) o2) e)))
            (ensures eq (merge l (do a o1) (do (do b o2') o2)) (do (merge l (do a o1) (do b o2')) o2)) = ()
 
-let rc_ind_left (l a b:concrete_st) (o1 o1' o2:op_t)
+let rc_ind_left' (l a b:concrete_st) (o1 o1' o2:op_t)
   : Lemma (requires Fst_then_snd? (rc o1 o2) /\
-                    eq (merge l (do a o1) (do b o2)) (do (merge l (do a o1) b) o2))
+                    eq (merge l (do a o1) (do b o2)) (do (merge l (do a o1) b) o2) /\
+                    (forall e. eq_e (sel_e (merge l (do (do a o1') o1) (do b o2)) e) (sel_e (do (merge l (do (do a o1') o1) b) o2) e)))
           (ensures eq (merge l (do (do a o1') o1) (do b o2)) (do (merge l (do (do a o1') o1) b) o2)) = ()
 
 //Special case of rc_intermediate_v1
-let rc_base (l:concrete_st) (o o1 o2:op_t)
+let rc_base' (l:concrete_st) (o o1 o2:op_t)
   : Lemma (requires Fst_then_snd? (rc o1 o2) /\ 
-                    eq (merge l (do l o1) (do l o2)) (do (do l o1) o2))
+                    eq (merge l (do l o1) (do l o2)) (do (do l o1) o2) /\
+                    (forall e. eq_e (sel_e (merge (do l o) (do (do l o) o1) (do (do l o) o2)) e) (sel_e (do (do (do l o) o1) o2) e)))
           (ensures eq (merge (do l o) (do (do l o) o1) (do (do l o) o2)) (do (do (do l o) o1) o2)) = ()
 
-let rc_base_base (o1 o2:op_t)
+let rc_base_base' (o1 o2:op_t)
   : Lemma (requires Fst_then_snd? (rc o1 o2))
           (ensures eq (merge init_st (do init_st o1) (do init_st o2)) (do (do init_st o1) o2)) = ()
 
-let rc_intermediate_base_right (l s1 s2 s3:concrete_st) (o o' o1 o2:op_t) 
-  : Lemma (requires Fst_then_snd? (rc o o') /\ Fst_then_snd? (rc o1 o2)
-                    /\ eq (merge (do l o') (do (do s1 o') o1) (do (do s2 o') o2)) (do (do (do s3 o') o1) o2)
-                    /\ eq (merge l (do s1 o1) (do s2 o2)) (do (do s3 o1) o2) 
-                    /\ eq (merge (do l o) (do (do l o) o1) (do (do l o) o2)) (do (do (do l o) o1) o2) //***EXTRA*** (from rc_base)
-                    /\ eq (merge l (do s1 o') (do s2 o)) (do (do s3 o) o')) //***EXTRA*** 
-          (ensures eq (merge (do l o') (do (do s1 o') o1) (do (do (do s2 o) o') o2)) (do (do (do (do s3 o) o') o1) o2)) =
+let rc_intermediate_base_right' (l s1 s2 s3:concrete_st) (o o' o1 o2:op_t) 
+  : Lemma (requires distinct_ops o o' /\ Fst_then_snd? (rc o o') /\ 
+                    distinct_ops o1 o2 /\ Fst_then_snd? (rc o1 o2) /\
+                    eq (merge (do l o') (do (do s1 o') o1) (do (do s2 o') o2)) (do (do (do s3 o') o1) o2) /\
+                    eq (merge l (do s1 o1) (do s2 o2)) (do (do s3 o1) o2) /\
+                    eq (merge l (do s1 o') (do s2 o)) (do (do s3 o) o') /\ //***EXTRA***
+                    (forall e. eq_e (sel_e (merge (do l o') (do (do s1 o') o1) (do (do (do s2 o) o') o2)) e)
+                               (sel_e (do (do (do (do s3 o) o') o1) o2) e)))
+          (ensures eq (merge (do l o') (do (do s1 o') o1) (do (do (do s2 o) o') o2)) (do (do (do (do s3 o) o') o1) o2)) = ()
+  (*if get_ele o2 = get_ele o' && get_rid o2 = get_rid o' then () //done
+  else if get_ele o2 = get_ele o' && get_rid o2 <> get_rid o' then () //done
+  else if get_ele o2 <> get_ele o' && get_rid o2 = get_rid o' then () //done
+  else () //done*)
+
+let rc_intermediate_base_left_right' (l s1 s2 s3:concrete_st) (o o' o1' o1 o2:op_t) 
+  : Lemma (requires distinct_ops o o' /\ Fst_then_snd? (rc o o') /\  
+                    distinct_ops o1 o2 /\ Fst_then_snd? (rc o1 o2) /\
+                    distinct_ops o1' o' /\ Fst_then_snd? (rc o1' o') /\
+                    eq (merge (do l o') (do (do s1 o') o1) (do (do s2 o') o2)) (do (do (do s3 o') o1) o2) /\
+                    eq (merge l (do s1 o1) (do s2 o2)) (do (do s3 o1) o2) /\
+                    (forall e. eq_e (sel_e (merge (do l o') (do (do (do s1 o1') o') o1) (do (do (do s2 o) o') o2)) e)
+                               (sel_e (do (do (do (do (do s3 o1') o) o') o1) o2) e))) 
+        (ensures eq (merge (do l o') (do (do (do s1 o1') o') o1) (do (do (do s2 o) o') o2)) (do (do (do (do (do s3 o1') o) o') o1) o2)) = ()
+  (*if get_ele o2 = get_ele o' && get_rid o2 = get_rid o' then () //done
+  else if get_ele o2 = get_ele o' && get_rid o2 <> get_rid o' then () //done
+  else if get_ele o2 <> get_ele o' && get_rid o2 = get_rid o' then () //done
+  else () //done*)
+
+let rc_intermediate_2_right' (l s1 s2 s3:concrete_st) (o1 o2 o o':op_t) (o_n:op_t{~ (commutes_with o_n o)})
+  : Lemma (requires distinct_ops o1 o2 /\ Fst_then_snd? (rc o1 o2) /\  
+                    distinct_ops o o' /\ Fst_then_snd? (rc o o') /\
+                    get_rid o_n <> get_rid o' (*o_n,o' must be concurrent*) /\
+                    eq (merge (do l o') (do (do s1 o') o1) (do (do (do s2 o) o') o2)) (do (do (do (do s3 o) o') o1) o2) /\
+                    (forall e. eq_e (sel_e (merge (do l o') (do (do s1 o') o1) (do (do (do (do s2 o_n) o) o') o2)) e)
+                               (sel_e (do (do (do (do (do s3 o_n) o) o') o1) o2) e)))
+          (ensures eq (merge (do l o') (do (do s1 o') o1) (do (do (do (do s2 o_n) o) o') o2)) (do (do (do (do (do s3 o_n) o) o') o1) o2)) = ()
+  (*assert (Add? (snd (snd o_n)) /\ get_ele o_n = get_ele o');
   if get_ele o2 = get_ele o' && get_rid o2 = get_rid o' then () //done
   else if get_ele o2 = get_ele o' && get_rid o2 <> get_rid o' then () //done
   else if get_ele o2 <> get_ele o' && get_rid o2 = get_rid o' then () //done
-  else () //done
+  else () //done*)
 
-let rc_intermediate_base_left_right (l s1 s2 s3:concrete_st) (o o' o1' o1 o2:op_t) 
-  : Lemma (requires Fst_then_snd? (rc o o') /\ Fst_then_snd? (rc o1 o2) /\ Fst_then_snd? (rc o1' o')
-                    /\ Either? (rc o o1') //***EXTRA*** 
-                    /\ eq (merge (do l o') (do (do s1 o') o1) (do (do s2 o') o2)) (do (do (do s3 o') o1) o2)
-                    /\ eq (merge l (do s1 o1) (do s2 o2)) (do (do s3 o1) o2)) 
-        (ensures eq (merge (do l o') (do (do (do s1 o1') o') o1) (do (do (do s2 o) o') o2)) (do (do (do (do (do s3 o1') o) o') o1) o2)) = 
+let rc_intermediate_2_left' (l s1 s2 s3:concrete_st) (o1 o2 o o':op_t) (o_n:op_t{~ (commutes_with o_n o)})
+  : Lemma (requires distinct_ops o1 o2 /\ Fst_then_snd? (rc o1 o2) /\  
+                    distinct_ops o o' /\ Fst_then_snd? (rc o o') /\
+                    get_rid o_n <> get_rid o' (*o_n,o' must be concurrent*) /\
+                    eq (merge (do l o') (do (do (do s1 o) o') o1) (do (do s2 o') o2)) (do (do (do (do s3 o) o') o1) o2) /\
+                    (forall e. eq_e (sel_e (merge (do l o') (do (do (do (do s1 o_n) o) o') o1) (do (do s2 o') o2)) e)
+                              (sel_e (do (do (do (do (do s3 o_n) o) o') o1) o2) e)))
+      (ensures eq (merge (do l o') (do (do (do (do s1 o_n) o) o') o1) (do (do s2 o') o2)) (do (do (do (do (do s3 o_n) o) o') o1) o2)) = ()
+  (*assert (Add? (snd (snd o_n)) /\ get_ele o_n = get_ele o');
   if get_ele o2 = get_ele o' && get_rid o2 = get_rid o' then () //done
   else if get_ele o2 = get_ele o' && get_rid o2 <> get_rid o' then () //done
   else if get_ele o2 <> get_ele o' && get_rid o2 = get_rid o' then () //done
-  else () //done
+  else () //done*)
 
-let rc_intermediate_2_right (l s1 s2 s3:concrete_st) (o1 o2:op_t) (o o':op_t) (o_n:op_t{~ (commutes_with o_n o)})
-: Lemma (requires Fst_then_snd? (rc o1 o2) /\ Fst_then_snd? (rc o o') /\
-                  //get_rid o <> get_rid o' (*o,o' must be concurrent *) /\
-                  get_rid o_n <> get_rid o' (*o_n,o' must be concurrent*) /\
-                  eq (merge (do l o') (do (do s1 o') o1) (do (do (do s2 o) o') o2)) (do (do (do (do s3 o) o') o1) o2))
-      (ensures eq (merge (do l o') (do (do s1 o') o1) (do (do (do (do s2 o_n) o) o') o2)) (do (do (do (do (do s3 o_n) o) o') o1) o2)) = 
-  assert (Add? (snd (snd o_n)) /\ get_ele o_n = get_ele o');
-  if get_ele o2 = get_ele o' && get_rid o2 = get_rid o' then () //done
-  else if get_ele o2 = get_ele o' && get_rid o2 <> get_rid o' then () //done
-  else if get_ele o2 <> get_ele o' && get_rid o2 = get_rid o' then () //done
-  else () //done
-
-let rc_intermediate_2_left (l s1 s2 s3:concrete_st) (o1 o2:op_t) (o o':op_t) (o_n:op_t{~ (commutes_with o_n o)})
-: Lemma (requires Fst_then_snd? (rc o1 o2) /\ Fst_then_snd? (rc o o') /\
-                  //get_rid o <> get_rid o' (*o,o' must be concurrent *) /\
-                  get_rid o_n <> get_rid o' (*o_n,o' must be concurrent*) /\
-                  eq (merge (do l o') (do (do (do s1 o) o') o1) (do (do s2 o') o2)) (do (do (do (do s3 o) o') o1) o2))
-      (ensures eq (merge (do l o') (do (do (do (do s1 o_n) o) o') o1) (do (do s2 o') o2)) (do (do (do (do (do s3 o_n) o) o') o1) o2)) =
-  assert (Add? (snd (snd o_n)) /\ get_ele o_n = get_ele o');
-  if get_ele o2 = get_ele o' && get_rid o2 = get_rid o' then () //done
-  else if get_ele o2 = get_ele o' && get_rid o2 <> get_rid o' then () //done
-  else if get_ele o2 <> get_ele o' && get_rid o2 = get_rid o' then () //done
-  else () //done
-
-let rc_intermediate_1_v2 (l s1 s2 s3:concrete_st) (o1 o2:op_t) (o':op_t{Add? (snd (snd o'))}) (o_n:op_t{Add? (snd (snd o_n))})
-  : Lemma (requires Fst_then_snd? (rc o1 o2) /\ 
-                    //get_rid o1 <> get_rid o2 /\
+let rc_intermediate_1_v2' (l s1 s2 s3:concrete_st) (o1 o2 o' o_n:op_t)
+  : Lemma (requires distinct_ops o1 o2 /\ Fst_then_snd? (rc o1 o2) /\ 
+                    (exists o. Fst_then_snd? (rc o o')) /\ (exists o. Fst_then_snd? (rc o o_n)) /\ 
                     eq (merge (do l o_n) (do (do s1 o_n) o1) (do (do s2 o_n) o2)) (do (do (do s3 o_n) o1) o2) /\
-                    eq (merge (do l o') (do (do s1 o') o1) (do (do s2 o') o2)) (do (do (do s3 o') o1) o2))
-    (ensures eq (merge (do (do l o_n) o') (do (do (do s1 o_n) o') o1) (do (do (do s2 o_n) o') o2)) (do (do (do (do s3 o_n) o') o1) o2)) =
-  if get_ele o2 = get_ele o' && get_rid o2 = get_rid o' then admit() //not done
-  else if get_ele o2 = get_ele o' && get_rid o2 <> get_rid o' then admit() //not done
-  else if get_ele o2 <> get_ele o' && get_rid o2 = get_rid o' then admit() //not done
-  else admit() //not done
+                    eq (merge (do l o') (do (do s1 o') o1) (do (do s2 o') o2)) (do (do (do s3 o') o1) o2) /\
+                    (forall e. eq_e (sel_e (merge (do (do l o_n) o') (do (do (do s1 o_n) o') o1) (do (do (do s2 o_n) o') o2)) e)
+                               (sel_e (do (do (do (do s3 o_n) o') o1) o2) e)))
+    (ensures eq (merge (do (do l o_n) o') (do (do (do s1 o_n) o') o1) (do (do (do s2 o_n) o') o2)) (do (do (do (do s3 o_n) o') o1) o2)) = ()
 
 (*One op*)
 ///////////////
-let ind_right_one_op (l a b c:concrete_st) (o1 o1':op_t)
+let ind_right_one_op' (l a b c:concrete_st) (o1 o1':op_t)
    : Lemma (requires eq (merge l a (do b o1)) (do (merge l a b) o1))
            (ensures eq (merge l a (do (do b o1') o1)) (do (merge l a (do b o1')) o1)) = ()
            
-let base_one_op (l:concrete_st) (o o1:op_t)
+let base_one_op' (l:concrete_st) (o o1:op_t)
   : Lemma (requires eq (merge l l (do l o1)) (do l o1))
           (ensures eq (merge (do l o) (do l o) (do (do l o) o1)) (do (do l o) o1) ) = ()
 
-let base_base_one_op (o1:op_t)
+let base_base_one_op' (o1:op_t)
   : Lemma (ensures eq (merge init_st init_st (do init_st o1)) (do init_st o1)) = ()
 
-let intermediate_base_right_one_op_right (l s1 s2 s3:concrete_st) (o o' o1:op_t) 
-  : Lemma (requires Fst_then_snd? (rc o o') 
-                    /\ eq (merge (do l o') (do s1 o') (do (do s2 o') o1)) (do (do s3 o') o1)
-                    /\ eq (merge l s1 (do s2 o1)) (do s3 o1)
-                    /\ eq (merge l (do s1 o') (do s2 o)) (do (do s3 o) o')) //***EXTRA***
+let intermediate_base_right_one_op' (l s1 s2 s3:concrete_st) (o o' o1:op_t) 
+  : Lemma (requires distinct_ops o o' /\ Fst_then_snd? (rc o o') /\
+                    eq (merge (do l o') (do s1 o') (do (do s2 o') o1)) (do (do s3 o') o1) /\
+                    eq (merge l s1 (do s2 o1)) (do s3 o1) /\
+                    eq (merge l (do s1 o') (do s2 o)) (do (do s3 o) o') /\ //***EXTRA***
+                    (forall e. eq_e (sel_e (merge (do l o') (do s1 o') (do (do (do s2 o) o') o1)) e) (sel_e (do (do (do s3 o) o') o1) e)))
           (ensures eq (merge (do l o') (do s1 o') (do (do (do s2 o) o') o1)) (do (do (do s3 o) o') o1)) = ()
 
-let intermediate_base_right_one_op_left (l s1 s2 s3:concrete_st) (o o' o1:op_t) 
-  : Lemma (requires Fst_then_snd? (rc o o') 
-                    /\ eq (merge (do l o') (do (do s1 o') o1) (do s2 o')) (do (do s3 o') o1)
-                    /\ eq (merge l (do s1 o1) s2) (do s3 o1)
-                    /\ eq (merge (do l o') (do (do l o') o1) (do (do l o) o')) (do (do (do l o) o') o1) //**EXTRA***
-                    /\ eq (merge l (do s1 o') (do s2 o)) (do (do s3 o) o')) //***EXTRA***
-          (ensures eq (merge (do l o') (do (do s1 o') o1) (do (do s2 o) o')) (do (do (do s3 o) o') o1)) = 
-  let lhs = (merge (do l o') (do (do s1 o') o1) (do (do s2 o) o')) in
+let intermediate_base_right_one_op_left' (l s1 s2 s3:concrete_st) (o o' o1:op_t) 
+  : Lemma (requires distinct_ops o o' /\ Fst_then_snd? (rc o o') /\ distinct_ops o' o1 /\
+                    eq (merge (do l o') (do (do s1 o') o1) (do s2 o')) (do (do s3 o') o1) /\
+                    (Fst_then_snd? (rc o o1) ==> eq (merge l (do s1 o1) (do s2 o)) (do (merge l s1 (do s2 o)) o1)) /\ //***EXTRA***       
+                    eq (merge l (do s1 o1) s2) (do s3 o1) /\
+                    eq (merge l (do s1 o') (do s2 o)) (do (do s3 o) o') /\ //***EXTRA***
+                    (forall e. eq_e (sel_e (merge (do l o') (do (do s1 o') o1) (do (do s2 o) o')) e) (sel_e (do (do (do s3 o) o') o1) e)))
+          (ensures eq (merge (do l o') (do (do s1 o') o1) (do (do s2 o) o')) (do (do (do s3 o) o') o1)) = ()
+  (*let lhs = (merge (do l o') (do (do s1 o') o1) (do (do s2 o) o')) in
   let rhs = (do (do (do s3 o) o') o1) in
   
   if Add? (snd (snd o1)) && get_ele o1 = get_ele o' && get_rid o1 = get_rid o' then () //done
@@ -263,34 +268,35 @@ let intermediate_base_right_one_op_left (l s1 s2 s3:concrete_st) (o o' o1:op_t)
   else if Add? (snd (snd o1)) && get_ele o1 <> get_ele o' && get_rid o1 = get_rid o' then () //done
   else if Add? (snd (snd o1)) && get_ele o1 <> get_ele o' && get_rid o1 <> get_rid o' then () //done
   else if Rem? (snd (snd o1)) && get_ele o1 = get_ele o' then ()
-  else ()
+  else ()*)
 
-let intermediate_base_left_one_op (l s1 s2 s3:concrete_st) (o o' o1:op_t) 
-  : Lemma (requires Fst_then_snd? (rc o o')  
-                    /\ eq (merge (do l o') (do s1 o') (do (do s2 o') o1)) (do (do s3 o') o1)
-                    /\ eq (merge l s1 (do s2 o1)) (do s3 o1) 
-                    /\ eq (merge l (do s1 o') (do s2 o)) (do (do s3 o) o') //***EXTRA***
-                    /\ eq (merge l (do (do s1 o) o') (do s2 o')) (do (do s3 o) o')) //***EXTRA***
-          (ensures eq (merge (do l o') (do (do s1 o) o') (do (do s2 o') o1)) (do (do (do s3 o) o') o1)) = 
-  if Add? (snd (snd o1)) && get_ele o1 = get_ele o' && get_rid o1 = get_rid o' then () //done
+let intermediate_base_left_one_op' (l s1 s2 s3:concrete_st) (o o' o1:op_t) 
+  : Lemma (requires distinct_ops o o' /\ Fst_then_snd? (rc o o') /\
+                    eq (merge (do l o') (do s1 o') (do (do s2 o') o1)) (do (do s3 o') o1) /\
+                    (Fst_then_snd? (rc o o1) ==> eq (merge l (do s1 o1) (do s2 o)) (do (merge l s1 (do s2 o)) o1)) /\ //***EXTRA***
+                    eq (merge l s1 (do s2 o1)) (do s3 o1) /\
+                    eq (merge l (do s1 o') (do s2 o)) (do (do s3 o) o') /\ //***EXTRA***
+                    eq (merge l (do (do s1 o) o') (do s2 o')) (do (do s3 o) o') /\ //***EXTRA***
+                    (forall e. eq_e (sel_e (merge (do l o') (do (do s1 o) o') (do (do s2 o') o1)) e)
+                               (sel_e (do (do (do s3 o) o') o1) e)))
+          (ensures eq (merge (do l o') (do (do s1 o) o') (do (do s2 o') o1)) (do (do (do s3 o) o') o1)) = ()
+  (*if Add? (snd (snd o1)) && get_ele o1 = get_ele o' && get_rid o1 = get_rid o' then () //done
   else if Add? (snd (snd o1)) && get_ele o1 = get_ele o' && get_rid o1 <> get_rid o' then () //done
   else if Add? (snd (snd o1)) && get_ele o1 <> get_ele o' && get_rid o1 = get_rid o' then () //done
   else if Add? (snd (snd o1)) && get_ele o1 <> get_ele o' && get_rid o1 <> get_rid o' then () //done
   else if Rem? (snd (snd o1)) && get_ele o1 = get_ele o' then () //done
-  else () //done
+  else () //done*)
 
-let intermediate_base_left_right_one_op (l s1 s2 s3:concrete_st) (o o' o1' o1:op_t) 
-  : Lemma (requires Fst_then_snd? (rc o o') /\ Fst_then_snd? (rc o1' o')
-                    ///\ get_rid o <> get_rid o' /\ get_rid o1' <> get_rid o' 
-                    /\ eq (merge (do l o1) (do (do l o1) o) (do (do l o1) o')) (do (do (do l o1) o) o') //***EXTRA*** (from rc_base)
-                    /\ eq (merge (do l o') (do s1 o') (do (do s2 o') o1)) (do (do s3 o') o1)
-                    /\ eq (merge (do l o') (do (do s1 o1') o') (do (do s2 o') o1)) (do (do (do s3 o1') o') o1) //EXTRA
-
-                    /\ eq (merge l s1 (do s2 o1)) (do s3 o1) 
-                    /\ eq (merge (do l o') (do (do l o') o1) (do (do l o) o')) (do (do (do l o) o') o1) //***EXTRA***
-                    /\ eq (merge (do l o') (do l o')  (do (do (do l o) o') o1)) (do (do (do l o) o') o1))
-          (ensures eq (merge (do l o') (do (do s1 o1') o') (do (do (do s2 o) o') o1)) (do (do (do (do s3 o1') o) o') o1)) = 
-  assert (Either? (rc o o1'));
+let intermediate_base_left_right_one_op' (l s1 s2 s3:concrete_st) (o o' o1' o1:op_t) 
+  : Lemma (requires distinct_ops o o' /\ Fst_then_snd? (rc o o') /\
+                    distinct_ops o1' o' /\ Fst_then_snd? (rc o1' o') /\
+                    eq (merge (do l o') (do s1 o') (do (do s2 o') o1)) (do (do s3 o') o1) /\
+                    eq (merge (do l o') (do (do s1 o1') o') (do (do s2 o') o1)) (do (do (do s3 o1') o') o1) /\ //EXTRA
+                    eq (merge l s1 (do s2 o1)) (do s3 o1) /\
+                    (forall e. eq_e (sel_e (merge (do l o') (do (do s1 o1') o') (do (do (do s2 o) o') o1)) e)
+                               (sel_e (do (do (do (do s3 o1') o) o') o1) e)))
+          (ensures eq (merge (do l o') (do (do s1 o1') o') (do (do (do s2 o) o') o1)) (do (do (do (do s3 o1') o) o') o1)) = ()
+  (*assert (Either? (rc o o1'));
   let lhs = (merge (do l o') (do (do s1 o1') o') (do (do (do s2 o) o') o1)) in
   let rhs = (do (do (do (do s3 o1') o) o') o1) in
   if Add? (snd (snd o1)) && get_ele o1 = get_ele o' && get_rid o1 = get_rid o' then () //done
@@ -301,162 +307,145 @@ let intermediate_base_left_right_one_op (l s1 s2 s3:concrete_st) (o o' o1' o1:op
   else if Add? (snd (snd o1)) && get_ele o1 <> get_ele o' && get_rid o1 = get_rid o' then () // done
   else if Add? (snd (snd o1)) && get_ele o1 <> get_ele o' && get_rid o1 <> get_rid o' then () // done
   else if Rem? (snd (snd o1)) && get_ele o1 = get_ele o' then () // done
-  else () // done
+  else () // done*)
 
-
-(*let intermediate_base_left_right_one_op_right (l s1 s2 s3:concrete_st) (o o' o1' o1:op_t) 
-  : Lemma (requires Fst_then_snd? (rc o o') /\ Fst_then_snd? (rc o1' o')
-                    /\ eq (merge (do l o') (do s1 o') (do (do s2 o') o1)) (do (do s3 o') o1)
-                    /\ eq (merge l s1 (do s2 o1)) (do s3 o1)
-                    /\ eq (merge (do l o') (do (do l o') o1) (do (do l o) o')) (do (do (do l o) o') o1)) //***EXTRA***
-          (ensures eq (merge (do l o') (do (do s1 o1') o') (do (do (do s2 o) o') o1)) (do (do (do (do s3 o1') o) o') o1)) = admit()
-
-let intermediate_base_left_right_one_op_left (l s1 s2 s3:concrete_st) (o o' o1' o1:op_t) 
-  : Lemma (requires Fst_then_snd? (rc o o') /\ Fst_then_snd? (rc o1' o')
-                    /\ eq (merge (do l o') (do (do s1 o') o1) (do s2 o')) (do (do s3 o') o1)
-                    /\ eq (merge l (do s1 o1) s2) (do s3 o1)
-                    /\ eq (merge (do l o') (do (do l o') o1) (do (do l o) o')) (do (do (do l o) o') o1)) //***EXTRA***
-          (ensures eq (merge (do l o') (do (do (do s1 o1') o') o1) (do (do s2 o) o')) (do (do (do (do s3 o1') o) o') o1)) = admit()*)
-
-let intermediate_2_right_one_op (l s1 s2 s3:concrete_st) (o1: op_t) (o o':op_t) (o_n:op_t{~ (commutes_with o_n o)})
-: Lemma (requires Fst_then_snd? (rc o o') /\
-                  //get_rid o <> get_rid o' (*o,o' must be concurrent *) /\
-                  get_rid o_n <> get_rid o' (*o_n,o' must be concurrent*) /\
-                  eq (merge (do l o') (do s1 o') (do (do (do s2 o) o') o1)) (do (do (do s3 o) o') o1))
-      (ensures eq (merge (do l o') (do s1 o') (do (do (do (do s2 o_n) o) o') o1)) (do (do (do (do s3 o_n) o) o') o1)) = 
-  assert (Add? (snd (snd o_n)) && get_ele o_n = get_ele o');
+let intermediate_2_left_one_op' (l s1 s2 s3:concrete_st) (o1 o o':op_t) (o_n:op_t{~ (commutes_with o_n o)})
+  : Lemma (requires distinct_ops o o' /\ Fst_then_snd? (rc o o') /\
+                    get_rid o_n <> get_rid o' (*o_n,o' must be concurrent*) /\
+                    eq (merge (do l o') (do (do s1 o) o') (do (do s2 o') o1)) (do (do (do s3 o) o') o1) /\
+                    (forall e. eq_e (sel_e (merge (do l o') (do (do (do s1 o_n) o) o') (do (do s2 o') o1)) e)
+                               (sel_e (do (do (do (do s3 o_n) o) o') o1) e)))
+      (ensures eq (merge (do l o') (do (do (do s1 o_n) o) o') (do (do s2 o') o1)) (do (do (do (do s3 o_n) o) o') o1)) = ()
+  (*assert (Add? (snd (snd o_n)) && get_ele o_n = get_ele o');
   if Add? (snd (snd o1)) && get_ele o1 = get_ele o' && get_rid o1 = get_rid o' then () //done
   else if Add? (snd (snd o1)) && get_ele o1 = get_ele o' && get_rid o1 <> get_rid o' then () //done
   else if Add? (snd (snd o1)) && get_ele o1 <> get_ele o' && get_rid o1 = get_rid o' then () //done
   else if Add? (snd (snd o1)) && get_ele o1 <> get_ele o' && get_rid o1 <> get_rid o' then () //done
   else if Rem? (snd (snd o1)) && get_ele o1 = get_ele o' then () //done
-  else () //done
-
-let intermediate_2_left_one_op (l s1 s2 s3:concrete_st) (o1:op_t) (o o':op_t) (o_n:op_t{~ (commutes_with o_n o)})
-: Lemma (requires Fst_then_snd? (rc o o') /\
-                  //get_rid o <> get_rid o' (*o,o' must be concurrent *) /\
-                  get_rid o_n <> get_rid o' (*o_n,o' must be concurrent*) /\
-                  eq (merge (do l o') (do (do s1 o) o') (do (do s2 o') o1)) (do (do (do s3 o) o') o1))
-      (ensures eq (merge (do l o') (do (do (do s1 o_n) o) o') (do (do s2 o') o1)) (do (do (do (do s3 o_n) o) o') o1)) = 
-  assert (Add? (snd (snd o_n)) && get_ele o_n = get_ele o');
-  if Add? (snd (snd o1)) && get_ele o1 = get_ele o' && get_rid o1 = get_rid o' then () //done
-  else if Add? (snd (snd o1)) && get_ele o1 = get_ele o' && get_rid o1 <> get_rid o' then () //done
-  else if Add? (snd (snd o1)) && get_ele o1 <> get_ele o' && get_rid o1 = get_rid o' then () //done
-  else if Add? (snd (snd o1)) && get_ele o1 <> get_ele o' && get_rid o1 <> get_rid o' then () //done
-  else if Rem? (snd (snd o1)) && get_ele o1 = get_ele o' then () //done
-  else () //done
+  else () //done*)
 
 // In general, the events o',o_n, below should be such that these exists o, (rc o o')
-let intermediate_1_v2_one_op (l s1 s2 s3:concrete_st) (o1:op_t) (o':op_t{Add? (snd (snd o'))}) (o_n:op_t{Add? (snd (snd o_n))})
-  : Lemma (requires eq (merge (do l o_n) (do s1 o_n) (do (do s2 o_n) o1)) (do (do s3 o_n) o1) /\
-                    eq (merge (do l o') (do s1 o') (do (do s2 o') o1)) (do (do s3 o') o1))
-          (ensures eq (merge (do (do l o_n) o') (do (do s1 o_n) o') (do (do (do s2 o_n) o') o1)) (do (do (do s3 o_n) o') o1)) = admit()
+let intermediate_1_v2_one_op' (l s1 s2 s3:concrete_st) (o1 o' o_n:op_t)
+  : Lemma (requires (exists o. Fst_then_snd? (rc o o')) /\ (exists o. Fst_then_snd? (rc o o_n)) /\ 
+                    eq (merge (do l o_n) (do s1 o_n) (do (do s2 o_n) o1)) (do (do s3 o_n) o1) /\
+                    eq (merge (do l o') (do s1 o') (do (do s2 o') o1)) (do (do s3 o') o1) /\
+                    (forall e. eq_e (sel_e (merge (do (do l o_n) o') (do (do s1 o_n) o') (do (do (do s2 o_n) o') o1)) e)
+                               (sel_e (do (do (do s3 o_n) o') o1) e)))
+          (ensures eq (merge (do (do l o_n) o') (do (do s1 o_n) o') (do (do (do s2 o_n) o') o1)) (do (do (do s3 o_n) o') o1)) = ()
 
 (*Zero op *)
 ///////////////
-let intermediate_base_right_zero_op (l s1 s2 s3:concrete_st) (o o':op_t) 
-  : Lemma (requires Fst_then_snd? (rc o o')  
-                    /\ eq (merge (do l o') (do s1 o') (do s2 o')) (do s3 o')
-                    /\ eq (merge l s1 s2) s3
-                    /\ eq (merge l (do s1 o') (do s2 o)) (do (do s3 o) o')) //***EXTRA***
+let intermediate_base_right_zero_op' (l s1 s2 s3:concrete_st) (o o':op_t) 
+  : Lemma (requires distinct_ops o o' /\ Fst_then_snd? (rc o o') /\
+                    eq (merge (do l o') (do s1 o') (do s2 o')) (do s3 o') /\
+                    eq (merge l s1 s2) s3 /\
+                    eq (merge l (do s1 o') (do s2 o)) (do (do s3 o) o') /\ //***EXTRA***
+                    (forall e. eq_e (sel_e (merge (do l o') (do s1 o') (do (do s2 o) o')) e) (sel_e (do (do s3 o) o') e)))
           (ensures eq (merge (do l o') (do s1 o') (do (do s2 o) o')) (do (do s3 o) o')) = ()
 
-let intermediate_base_left_right_zero_op (l s1 s2 s3:concrete_st) (o o' o1':op_t) 
-  : Lemma (requires Fst_then_snd? (rc o o') /\ Fst_then_snd? (rc o1' o')
-                    /\ eq (merge (do l o') (do s1 o') (do s2 o')) (do s3 o')
-                    /\ eq (merge l s1 s2) s3 ) 
+let intermediate_base_left_right_zero_op' (l s1 s2 s3:concrete_st) (o o' o1':op_t) 
+  : Lemma (requires distinct_ops o o' /\ Fst_then_snd? (rc o o') /\  
+                    distinct_ops o1' o' /\ Fst_then_snd? (rc o1' o') /\
+                    eq (merge (do l o') (do s1 o') (do s2 o')) (do s3 o') /\
+                    eq (merge l s1 s2) s3 /\
+                    (forall e. eq_e (sel_e (merge (do l o') (do (do s1 o1') o') (do (do s2 o) o')) e)
+                               (sel_e (do (do (do s3 o1') o) o') e)))
           (ensures eq (merge (do l o') (do (do s1 o1') o') (do (do s2 o) o')) (do (do (do s3 o1') o) o')) = ()
 
-let intermediate_2_right_zero_op (l s1 s2 s3:concrete_st) (o o':op_t) (o_n:op_t{~ (commutes_with o_n o)})
-: Lemma (requires Fst_then_snd? (rc o o') /\
-                  //get_rid o <> get_rid o' (*o,o' must be concurrent *) /\
-                  get_rid o_n <> get_rid o' (*o_n,o' must be concurrent*) /\
-                  eq (merge (do l o') (do s1 o') (do (do s2 o) o')) (do (do s3 o) o'))
-      (ensures eq (merge (do l o') (do s1 o') (do (do (do s2 o_n) o) o')) (do (do (do s3 o_n) o) o')) = 
-  assert (Fst_then_snd? (rc o o_n) && get_ele o = get_ele o_n);
+let intermediate_2_right_zero_op' (l s1 s2 s3:concrete_st) (o o':op_t) (o_n:op_t{~ (commutes_with o_n o)})
+  : Lemma (requires distinct_ops o o' /\ Fst_then_snd? (rc o o') /\
+                    get_rid o_n <> get_rid o' (*o_n,o' must be concurrent*) /\
+                    eq (merge (do l o') (do s1 o') (do (do s2 o) o')) (do (do s3 o) o') /\
+                    (forall e. eq_e (sel_e (merge (do l o') (do s1 o') (do (do (do s2 o_n) o) o')) e) (sel_e (do (do (do s3 o_n) o) o') e)))
+      (ensures eq (merge (do l o') (do s1 o') (do (do (do s2 o_n) o) o')) (do (do (do s3 o_n) o) o')) = ()
+  (*assert (Fst_then_snd? (rc o o_n) && get_ele o = get_ele o_n);
   assert (Either? (rc o' o_n));
   if get_ele o_n = get_ele o' then () //done
-  else ()
+  else ()*)
 
-let intermediate_2_left_zero_op (l s1 s2 s3:concrete_st) (o o':op_t) (o_n:op_t{~ (commutes_with o_n o)})
-: Lemma (requires Fst_then_snd? (rc o o') /\
-                  //get_rid o <> get_rid o' (*o,o' must be concurrent *) /\
-                  get_rid o_n <> get_rid o' (*o_n,o' must be concurrent*) /\
-                  eq (merge (do l o') (do (do s1 o) o') (do s2 o')) (do (do s3 o) o'))
-      (ensures eq (merge (do l o') (do (do (do s1 o_n) o) o') (do s2 o')) (do (do (do s3 o_n) o) o')) = 
-  assert (Fst_then_snd? (rc o o_n) && get_ele o = get_ele o_n);
+let intermediate_2_left_zero_op' (l s1 s2 s3:concrete_st) (o o':op_t) (o_n:op_t{~ (commutes_with o_n o)})
+  : Lemma (requires distinct_ops o o' /\ Fst_then_snd? (rc o o') /\
+                    get_rid o_n <> get_rid o' (*o_n,o' must be concurrent*) /\
+                    eq (merge (do l o') (do (do s1 o) o') (do s2 o')) (do (do s3 o) o') /\
+                    (forall e. eq_e (sel_e (merge (do l o') (do (do (do s1 o_n) o) o') (do s2 o')) e) (sel_e (do (do (do s3 o_n) o) o') e)))
+      (ensures eq (merge (do l o') (do (do (do s1 o_n) o) o') (do s2 o')) (do (do (do s3 o_n) o) o')) = ()
+  (*assert (Fst_then_snd? (rc o o_n) && get_ele o = get_ele o_n);
   assert (Either? (rc o' o_n));
   if get_ele o_n = get_ele o' then () //done
-  else ()
+  else ()*)
 
 // In general, the event "o" below should be such that these exists o', (rc o' o)
-let intermediate_1_v1_zero_op (l s1 s2 s3:concrete_st) (o:op_t{Add? (snd (snd o))})
-  : Lemma (requires eq (merge l s1 s2) s3)
+let intermediate_1_v1_zero_op' (l s1 s2 s3:concrete_st) (o:op_t)
+  : Lemma (requires (exists o'. Fst_then_snd? (rc o' o)) /\ eq (merge l s1 s2) s3)
           (ensures eq (merge (do l o) (do s1 o) (do s2 o)) (do s3 o) ) = ()
 
 // In general, the events o',o_n, below should be such that these exists o, (rc o o')
-let intermediate_1_v2_zero_op (l s1 s2 s3:concrete_st) (o':op_t{Add? (snd (snd o'))}) (o_n:op_t{Add? (snd (snd o_n))})
-  : Lemma (requires eq (merge (do l o_n) (do s1 o_n) (do s2 o_n)) (do s3 o_n)  /\
-                    eq (merge (do l o') (do s1 o') (do s2 o')) (do s3 o'))
+let intermediate_1_v2_zero_op' (l s1 s2 s3:concrete_st) (o' o_n:op_t)
+  : Lemma (requires (exists o. Fst_then_snd? (rc o o')) /\ (exists o. Fst_then_snd? (rc o o_n)) /\ 
+                    eq (merge (do l o_n) (do s1 o_n) (do s2 o_n)) (do s3 o_n)  /\
+                    eq (merge (do l o') (do s1 o') (do s2 o')) (do s3 o') /\
+                    (forall e. eq_e (sel_e (merge (do (do l o_n) o') (do (do s1 o_n) o') (do (do s2 o_n) o')) e)
+                               (sel_e (do (do s3 o_n) o') e)))
           (ensures eq (merge (do (do l o_n) o') (do (do s1 o_n) o') (do (do s2 o_n) o')) (do (do s3 o_n) o')) = ()
 
 (* 2 op Comm  *)
 ///////////////////
 
-let comm_ind_right (l a b c:concrete_st) (o1 o2' o2:op_t)
-  : Lemma (requires Either? (rc o1 o2) /\
-                    //commutes_with o1 o2 /\
+let comm_ind_right' (l a b c:concrete_st) (o1 o2' o2:op_t)
+  : Lemma (requires distinct_ops o1 o2 /\ Either? (rc o1 o2) /\ distinct_ops o2' o1 /\
                     eq (merge l (do a o1) (do b o2)) (do (do (merge l a b) o2) o1) /\
                     (Fst_then_snd? (rc o2' o1) ==> (eq (merge l (do a o1) (do b o2')) (do (merge l a (do b o2')) o1))) /\
-                    //~ (exists o3 a'. eq (do a o1) (do a' o3) /\ distinct_ops o2 o3 /\ Fst_then_snd? (rc o2 o3)) /\
-                    ~ (Fst_then_snd? (rc o1 o2')) )
-                    //~ (exists o3 b'. eq (do (do b o2') o2) (do b' o3) /\ distinct_ops o1 o3 /\ Fst_then_snd? (rc o1 o3)) /\
-                    //~ (exists o3 b'. eq (do b o2) (do b' o3) /\ distinct_ops o1 o3 /\ Fst_then_snd? (rc o1 o3)))                    
-          (ensures eq (merge l (do a o1) (do (do b o2') o2)) (do (do (merge l a (do b o2')) o2) o1)) = 
-  if Add? (snd (snd o1)) && Add? (snd (snd o2)) && get_ele o1 = get_ele o2 then () //done
+                    ~ (exists o3 a'. eq (do a o1) (do a' o3) /\ distinct_ops o2 o3 /\ Fst_then_snd? (rc o2 o3)) /\
+                    ~ (Fst_then_snd? (rc o1 o2')) /\
+                    ~ (exists o3 b'. eq (do (do b o2') o2) (do b' o3) /\ distinct_ops o1 o3 /\ Fst_then_snd? (rc o1 o3)) /\
+                    ~ (exists o3 b'. eq (do b o2) (do b' o3) /\ distinct_ops o1 o3 /\ Fst_then_snd? (rc o1 o3)) /\
+                    (forall e. eq_e (sel_e (merge l (do a o1) (do (do b o2') o2)) e) (sel_e (do (do (merge l a (do b o2')) o2) o1) e)))      
+          (ensures eq (merge l (do a o1) (do (do b o2') o2)) (do (do (merge l a (do b o2')) o2) o1)) = ()
+  (*if Add? (snd (snd o1)) && Add? (snd (snd o2)) && get_ele o1 = get_ele o2 then () //done
   else if Add? (snd (snd o1)) && Add? (snd (snd o2)) && get_ele o1 <> get_ele o2 && Add? (snd (snd o2')) then () //done
   else if Add? (snd (snd o1)) && Add? (snd (snd o2)) && get_ele o1 <> get_ele o2 && Rem? (snd (snd o2')) then () //done
   else if Add? (snd (snd o1)) && Rem? (snd (snd o2)) then () //done
   else if Rem? (snd (snd o1)) && Add? (snd (snd o2)) then () //done
-  else ()
+  else ()*)
 
-let comm_ind_left (l a b c:concrete_st) (o1 o2' o2:op_t)
-  : Lemma (requires Either? (rc o1 o2) /\
-                    //commutes_with o1 o2 /\
+let comm_ind_left' (l a b c:concrete_st) (o1 o2' o2:op_t)
+  : Lemma (requires distinct_ops o1 o2 /\ Either? (rc o1 o2) /\ distinct_ops o2' o2 /\
                     eq (merge l (do a o1) (do b o2)) (do (do (merge l a b) o2) o1) /\
                     (Fst_then_snd? (rc o2' o2) ==> (eq (merge l (do a o2') (do b o2)) (do (merge l (do a o2') b) o2))) /\
-                    //~ (exists o3 a'. eq (do a o1) (do a' o3) /\ distinct_ops o2 o3 /\ Fst_then_snd? (rc o2 o3)) /\
-                    ~ (Fst_then_snd? (rc o2 o2')) )
-                    //~ (exists o3 b'. eq (do (do b o2') o2) (do b' o3) /\ distinct_ops o1 o3 /\ Fst_then_snd? (rc o1 o3)) /\
-                    //~ (exists o3 b'. eq (do b o2) (do b' o3) /\ distinct_ops o1 o3 /\ Fst_then_snd? (rc o1 o3)))                    
-          (ensures eq (merge l (do (do a o2') o1) (do b o2)) (do (do (merge l (do a o2') b) o2) o1)) = 
-  if Add? (snd (snd o1)) && Add? (snd (snd o2)) && get_ele o1 = get_ele o2 then () //done
+                    ~ (exists o3 a'. eq (do a o1) (do a' o3) /\ distinct_ops o2 o3 /\ Fst_then_snd? (rc o2 o3)) /\
+                    ~ (Fst_then_snd? (rc o2 o2')) /\
+                    ~ (exists o3 b'. eq (do (do b o2') o2) (do b' o3) /\ distinct_ops o1 o3 /\ Fst_then_snd? (rc o1 o3)) /\
+                    ~ (exists o3 b'. eq (do b o2) (do b' o3) /\ distinct_ops o1 o3 /\ Fst_then_snd? (rc o1 o3)) /\
+                    (forall e. eq_e (sel_e (merge l (do (do a o2') o1) (do b o2)) e) (sel_e (do (do (merge l (do a o2') b) o2) o1) e)))      
+          (ensures eq (merge l (do (do a o2') o1) (do b o2)) (do (do (merge l (do a o2') b) o2) o1)) = ()
+  (*if Add? (snd (snd o1)) && Add? (snd (snd o2)) && get_ele o1 = get_ele o2 then () //done
   else if Add? (snd (snd o1)) && Add? (snd (snd o2)) && get_ele o1 <> get_ele o2 && Add? (snd (snd o2')) then () //done
   else if Add? (snd (snd o1)) && Add? (snd (snd o2)) && get_ele o1 <> get_ele o2 && Rem? (snd (snd o2')) then () //done
   else if Add? (snd (snd o1)) && Rem? (snd (snd o2)) then () //done
   else if Rem? (snd (snd o1)) && Add? (snd (snd o2)) then () //done
-  else ()
+  else ()*)
 
-let comm_base (l:concrete_st) (o o1 o2:op_t)
-  : Lemma (requires Either? (rc o1 o2) /\
-                    //commutes_with o1 o2 /\
+let comm_base' (l:concrete_st) (o o1 o2:op_t)
+  : Lemma (requires distinct_ops o1 o2 /\ Either? (rc o1 o2) /\ distinct_ops o o1 /\ distinct_ops o o2 /\
                     eq (merge l (do l o1) (do l o2)) (do (do l o2) o1))
           (ensures eq (merge (do l o) (do (do l o) o1) (do (do l o) o2)) (do (do (do l o) o2) o1)) = ()
 
-let comm_base_base (o1 o2:op_t)
-  : Lemma (requires Either? (rc o1 o2))
+let comm_base_base' (o1 o2:op_t)
+  : Lemma (requires distinct_ops o1 o2 /\ Either? (rc o1 o2))
           (ensures eq (merge init_st (do init_st o1) (do init_st o2)) (do (do init_st o1) o2)) = ()
 
-let comm_intermediate_base_right (l s1 s2 s3:concrete_st) (o o' o1 o2:op_t) 
-  : Lemma (requires //Fst_then_snd? (rc o o') /\ Either? (rc o1 o2)
-                    Rem? (snd (snd o)) /\ Add? (snd (snd o')) /\ get_ele o = get_ele o' /\
-                    Add? (snd (snd o1)) /\ Add? (snd (snd o2))
-                    /\ eq (merge l (do s1 o1) (do (do s2 o) o2)) (do (do (merge l s1 (do s2 o)) o1) o2) //comes from comm_ind_right
-                    /\ eq (merge (do l o') (do (do s1 o') o1) (do (do s2 o') o2)) (do (do (do s3 o') o1) o2) 
-                    /\ eq (merge (do l o') (do s1 o') (do (do s2 o) o')) (do (do s3 o) o') //comes from intermediate_base_zero_op
-                    /\ eq (merge l (do s1 o1) (do s2 o2)) (do (do s3 o1) o2)) 
-          (ensures eq (merge (do l o') (do (do s1 o') o1) (do (do (do s2 o) o') o2)) (do (do (do (do s3 o) o') o1) o2)) = 
-  if Rem? (snd (snd o1)) && Rem? (snd (snd o2)) then admit() //done
+let comm_intermediate_base_right' (l s1 s2 s3:concrete_st) (o o' o1 o2:op_t) 
+  : Lemma (requires distinct_ops o o' /\ Fst_then_snd? (rc o o') /\ 
+                    distinct_ops o1 o2 /\ Either? (rc o1 o2) /\
+                    distinct_ops o' o1 /\ distinct_ops o' o2 /\
+                    eq (merge l (do s1 o1) (do (do s2 o) o2)) (do (do (merge l s1 (do s2 o)) o1) o2) /\ //comes from comm_ind_right
+                    eq (merge (do l o') (do (do s1 o') o1) (do (do s2 o') o2)) (do (do (do s3 o') o1) o2) /\ 
+                    eq (merge (do l o') (do s1 o') (do (do s2 o) o')) (do (do s3 o) o') /\ //comes from intermediate_base_zero_op
+                    eq (merge l (do s1 o1) (do s2 o2)) (do (do s3 o1) o2) /\
+                    (forall e. eq_e (sel_e (merge (do l o') (do (do s1 o') o1) (do (do (do s2 o) o') o2)) e)
+                               (sel_e (do (do (do (do s3 o) o') o1) o2) e)))
+          (ensures eq (merge (do l o') (do (do s1 o') o1) (do (do (do s2 o) o') o2)) (do (do (do (do s3 o) o') o1) o2)) = ()
+  (*if Rem? (snd (snd o1)) && Rem? (snd (snd o2)) then admit() //done
   else if Add? (snd (snd o1)) && Rem? (snd (snd o2)) && get_ele o1 = get_ele o' then admit() //done
   else if Add? (snd (snd o1)) && Rem? (snd (snd o2)) && get_ele o1 <> get_ele o' then admit() //done
   else if Rem? (snd (snd o1)) && Add? (snd (snd o2)) && get_ele o2 = get_ele o' then admit() //done
@@ -472,42 +461,58 @@ let comm_intermediate_base_right (l s1 s2 s3:concrete_st) (o o' o1 o2:op_t)
   else if get_ele o1 = get_ele o' && get_ele o2 <> get_ele o' && get_rid o1 <> get_rid o' && get_rid o2 = get_rid o' then admit() // done
   else if get_ele o1 = get_ele o' && get_ele o2 <> get_ele o' && get_rid o1 <> get_rid o' && get_rid o2 <> get_rid o' then admit() // not done
   
-  else admit() //not done
+  else admit() //not done*)
 
-let comm_intermediate_base_left_right (l s1 s2 s3:concrete_st) (o o' o1' o1 o2:op_t) 
-  : Lemma (requires Fst_then_snd? (rc o o') /\ Either? (rc o1 o2) /\ Fst_then_snd? (rc o1' o')
-                    /\ eq (merge (do l o') (do (do s1 o') o1) (do (do s2 o') o2)) (do (do (do s3 o') o1) o2)
-                    /\ eq (merge l (do s1 o1) (do s2 o2)) (do (do s3 o1) o2)  
-                    /\ eq (merge l (do (do s1 o1') o1) (do (do s2 o) o2)) (do (do (merge l (do s1 o1') (do s2 o)) o1) o2) //comes from comm_ind_right
-                    /\ eq (merge (do l o') (do s1 o') (do (do s2 o) o')) (do (do s3 o) o')) //comes from intermediate_base_zero_op
+let comm_intermediate_base_left_right' (l s1 s2 s3:concrete_st) (o o' o1' o1 o2:op_t) 
+  : Lemma (requires distinct_ops o o' /\ Fst_then_snd? (rc o o') /\ 
+                    distinct_ops o1 o2 /\ Either? (rc o1 o2) /\
+                    distinct_ops o1' o' /\ Fst_then_snd? (rc o1' o') /\
+                    distinct_ops o' o1 /\ distinct_ops o' o2 /\
+                    eq (merge (do l o') (do (do s1 o') o1) (do (do s2 o') o2)) (do (do (do s3 o') o1) o2) /\
+                    eq (merge l (do s1 o1) (do s2 o2)) (do (do s3 o1) o2) /\
+                    eq (merge l (do (do s1 o1') o1) (do (do s2 o) o2)) (do (do (merge l (do s1 o1') (do s2 o)) o1) o2) /\ //comes from comm_ind_right
+                    eq (merge (do l o') (do s1 o') (do (do s2 o) o')) (do (do s3 o) o') /\ //comes from intermediate_base_zero_op
+                    (forall e. eq_e (sel_e (merge (do l o') (do (do (do s1 o1') o') o1) (do (do (do s2 o) o') o2)) e)
+                               (sel_e (do (do (do (do (do s3 o1') o) o') o1) o2) e)))
+          (ensures eq (merge (do l o') (do (do (do s1 o1') o') o1) (do (do (do s2 o) o') o2)) (do (do (do (do (do s3 o1') o) o') o1) o2)) = ()
 
-        (ensures eq (merge (do l o') (do (do (do s1 o1') o') o1) (do (do (do s2 o) o') o2)) (do (do (do (do (do s3 o1') o) o') o1) o2)) = admit()
-
-let comm_intermediate_2_right (l s1 s2 s3:concrete_st) (o1 o2:op_t) (o o':op_t) (o_n:op_t)//{~ (commutes_with o_n o)})
-: Lemma (requires Either? (rc o1 o2) /\ Fst_then_snd? (rc o o') /\
-                  //get_rid o <> get_rid o' (*o,o' must be concurrent *) /\
-                  get_rid o_n <> get_rid o' (*o_n,o' must be concurrent*) /\
-                 // Either? (rc o_n o') /\ 
-                  eq (merge (do l o') (do (do s1 o') o1) (do (do (do s2 o) o') o2)) (do (do (do (do s3 o) o') o1) o2))
-      (ensures eq (merge (do l o') (do (do s1 o') o1) (do (do (do (do s2 o_n) o) o') o2)) (do (do (do (do (do s3 o_n) o) o') o1) o2)) = 
-  assume (Either? (rc o_n o') /\ Fst_then_snd? (rc o o') /\ get_ele o = get_ele o');
+let comm_intermediate_2_right' (l s1 s2 s3:concrete_st) (o1 o2 o o':op_t) (o_n:op_t{~ (commutes_with o_n o)})
+  : Lemma (requires distinct_ops o1 o2 /\ Either? (rc o1 o2) /\  
+                    distinct_ops o o' /\ Fst_then_snd? (rc o o') /\
+                    get_rid o_n <> get_rid o' (*o_n,o' must be concurrent*) /\
+                    distinct_ops o_n o' /\ Either? (rc o_n o') /\ 
+                    eq (merge (do l o') (do (do s1 o') o1) (do (do (do s2 o) o') o2)) (do (do (do (do s3 o) o') o1) o2) /\
+                    (forall e. eq_e (sel_e (merge (do l o') (do (do s1 o') o1) (do (do (do (do s2 o_n) o) o') o2)) e)
+                               (sel_e (do (do (do (do (do s3 o_n) o) o') o1) o2) e)))
+      (ensures eq (merge (do l o') (do (do s1 o') o1) (do (do (do (do s2 o_n) o) o') o2)) (do (do (do (do (do s3 o_n) o) o') o1) o2)) = ()
+  (*assume (Either? (rc o_n o') /\ Fst_then_snd? (rc o o') /\ get_ele o = get_ele o');
   let lhs = (merge (do l o') (do (do s1 o') o1) (do (do (do (do s2 o_n) o) o') o2)) in
   let rhs = (do (do (do (do (do s3 o_n) o) o') o1) o2) in
   assume (forall ele. M.contains lhs ele = M.contains rhs ele);
   assume (forall ele. M.contains lhs ele ==> (forall rid. M.contains (sel_e lhs ele) rid = M.contains (sel_e rhs ele) rid));
-  admit()
+  admit()*)
 
-#push-options "--z3rlimit 100 --max_ifuel 5 --split_queries always"
-let comm_intermediate_1_v1 (l s1 s2 s3:concrete_st) (o1 o2:op_t) (o:op_t{Add? (snd (snd o))})
-  : Lemma (requires Either? (rc o1 o2) /\
-                    eq (merge (do l o) (do (do l o) o1) (do (do l o) o2)) (do (do (do l o) o2) o1) /\ //***EXTRA***
-                    eq (merge l (do s1 o1) (do s2 o2)) (do (do s3 o1) o2))
-          (ensures eq (merge (do l o) (do (do s1 o) o1) (do (do s2 o) o2)) (do (do (do s3 o) o1) o2)) = 
-  let lhs = (merge (do l o) (do (do s1 o) o1) (do (do s2 o) o2)) in
+let comm_intermediate_2_left' (l s1 s2 s3:concrete_st) (o1 o2 o o':op_t) (o_n:op_t{~ (commutes_with o_n o)})
+  : Lemma (requires distinct_ops o1 o2 /\ Either? (rc o1 o2) /\  
+                    distinct_ops o o' /\ Fst_then_snd? (rc o o') /\
+                    get_rid o_n <> get_rid o' (*o_n,o' must be concurrent*) /\
+                    distinct_ops o_n o' /\ Either? (rc o_n o') /\ 
+                    eq (merge (do l o') (do (do (do s1 o) o') o1) (do (do s2 o') o2)) (do (do (do (do s3 o) o') o1) o2) /\
+                    (forall e. eq_e (sel_e (merge (do l o') (do (do (do (do s1 o_n) o) o') o1) (do (do s2 o') o2)) e)
+                               (sel_e (do (do (do (do (do s3 o_n) o) o') o1) o2) e)))
+          (ensures eq (merge (do l o') (do (do (do (do s1 o_n) o) o') o1) (do (do s2 o') o2)) (do (do (do (do (do s3 o_n) o) o') o1) o2)) = ()
+
+let comm_intermediate_1_v1' (l s1 s2 s3:concrete_st) (o1 o2 o:op_t)
+  : Lemma (requires distinct_ops o1 o2 /\ Either? (rc o1 o2) /\ distinct_ops o1 o /\ distinct_ops o o2 /\
+                    (exists o'. Fst_then_snd? (rc o' o)) /\
+                    eq (merge l (do s1 o1) (do s2 o2)) (do (do s3 o1) o2) /\
+                    (forall e. eq_e (sel_e (merge (do l o) (do (do s1 o) o1) (do (do s2 o) o2)) e) (sel_e (do (do (do s3 o) o1) o2) e)))
+          (ensures eq (merge (do l o) (do (do s1 o) o1) (do (do s2 o) o2)) (do (do (do s3 o) o1) o2)) = ()
+  (*let lhs = (merge (do l o) (do (do s1 o) o1) (do (do s2 o) o2)) in
   let rhs = (do (do (do s3 o) o1) o2) in
   assume (forall ele. M.contains lhs ele = M.contains rhs ele);
   assume (forall ele. M.contains lhs ele ==> (forall rid. M.contains (sel_e lhs ele) rid = M.contains (sel_e rhs ele) rid));
   assume (forall ele rid. (ele <> get_ele o /\ rid <> get_rid o) ==> ( (sel_id (sel_e lhs ele) rid) =  (sel_id (sel_e rhs ele) rid)));
   assume (forall ele rid. (ele <> get_ele o /\ rid = get_rid o) ==> (fst (sel_id (sel_e lhs ele) rid) = fst (sel_id (sel_e rhs ele) rid)));
   assert (forall ele rid. (ele = get_ele o /\ rid <> get_rid o) ==> (fst (sel_id (sel_e lhs ele) rid) = fst (sel_id (sel_e rhs ele) rid)));
-  admit()
+  admit()*)
